
\begin{theorem}[Kolmogorov's zeroâ€“one law]
	
	$$\mathcal{T}_n = \sigma (X_n, X_{n+1}, \dots)$$
	$$\mathcal{T} = \bigcap_n \mathcal{T}_n$$
	
	
	Suppose $\left\{ X_n\right\}_{n=1}^\infty$ are independent, then $\forall A\in \mathcal{T}$, $P(A) \in \left\{ 0,1\right\}$.
	
	\begin{proof}
		We show that $P(A)=P(A)^2$.
		
		We show that $\mathcal{T}$ is independent of itself, $\forall A,B \in \mathcal{T} \quad P(A\cup B) = P(A)\cdot P(B)$.
		
		$\mathcal{T} \subset \mathcal{T}_1$. Consider $\mathcal{I}_{l,n} = \sigma (X_l, X_{l+1}, \dots, X_n)$
		
		For $n<k$, take $A\in\mathcal{I}_{l,n} $, $B\in\mathcal{I}_{k,m} $, then $A$, $B$ are independent.
		
		Let $\Pi_n = \bigcup_{m>n+1} \mathcal{I}_{n+1,m}$. $\Pi_n$ is $\pi$-system, and $\sigma(\Pi_n) = \mathcal{T}_n$.
		
		By lemma \ref{ind_lemma}, $\mathcal{I}_{l,n} $ is independent on $\mathcal{T}_n$. Thus $\forall A \in \mathcal{I}_{l,n}$, $B \in \mathcal{T}_n$,
		$$P(A\cap B) = P(A) \cdot P(B)$$
		
		$\mathcal{T}_1 = \sigma\qty(\bigcup_n \mathcal{I}_{1,n})$, and thus $\mathcal{T}_1$ is independent from $\mathcal{T}$ and since $\mathcal{T} \subseteq \mathcal{T}_1$, thus $\mathcal{T}$ is independent of itself and 
		$$\forall A\in \mathcal{T} \quad P(A) = P(A\cap A) = P(A)^2 $$
		
	\end{proof}
	\begin{coll}
		If $\left\{ X_n\right\}_{n=1}^\infty$ i.i.d. $s_n = \sum_{i=1}^n X_i$ then $\forall c\in \mathbb{R} \quad P(\limsup \frac{S_n}{n}\geq c) \in \left\{ 0,1 \right\} $.
	\end{coll}
\end{theorem}


\begin{prop}
Let $\left\{ X_n\right\}_{n=1}^\infty$ i.i.d. $s_n = \sum_{i=1}^n X_i$ then $ P(\limsup \frac{S_n}{n} \text{ exists}) \in \left\{ 0,1 \right\} $.

If $ P(\limsup \frac{S_n}{n} \text{ exists}) = 1 $, then 
$\exists c \in [-\infty, \infty]$ such that $P(\limsup \frac{S_n}{n} = c) = 1$.
\end{prop}

\section{Integration theory}
\begin{definition}[Notation]
	$(S, \mathcal{F}, \mu)$. Given $f: S\to \mathbb{R}$ measurable. We define
	$$\mu(f) = \int\limits_S f(S) \dd{\mu(S)}$$
	If $A\in \mathcal{F}$:
	$$\mu(f_{j}A) =  \mu(f\cdot \mathds{1}_A) = \int_Af(S) \dd{\mu(S)} = \int_A f \dd{\mu} $$
\end{definition}
\paragraph{Desirable properties of integral}
\begin{enumerate}
	\item Linearity $$\int \alpha f + g \dd{\mu} = \alpha \int f \dd{\mu} + \int g \dd{\mu}$$
	\item Positivity: $$f>0 \Rightarrow \int f \dd{\mu}>0$$
	\item $$\int \mathds{1}_A \dd{\mu} = \mu(A)$$
\end{enumerate}

Classes of functions we are going to consider:
\begin{enumerate}
	\item $$\mathcal{S} = \left\{ f(x) = \sum_{k=1}^m a_k \mathds{1}_{A_k} \: a_k>0, A_k \in \mathcal{F} \right\}$$ 
	\item $$\mathcal{P} = \left\{\text{positive measurable functions} \right\}$$ 
	\item $$\mathcal{I} = \left\{ f(x) = g(x)-h(x) | \: g,h\in \mathcal{P}, \int g \dd{\mu}  \text{ or } \int h \dd{\mu}  \text{ finite.} \right\} $$ 
\end{enumerate}

\begin{definition}
	For $\phi \in \mathcal{S}$ let $\mu_0(\phi) = \int_S \phi(S) \dd{\mu_0}  =\sum_{k=1}^m a_k \mu(A_k)$.
\end{definition}

\begin{definition}
For $f \in \mathcal{P}$ let $\mu(\phi) = \sup\limits_{\substack{\phi \in \mathcal{S} \\ \phi\leq f}} \mu_0(\phi)$.
\end{definition}

\begin{prop}
	If $f=g$ $\mu$ a.e., then $\mu(f)=\mu(g)$.
\end{prop}

\begin{lemma}
	If $\mu(f) = 0$ then $f=0$ a.e.
\end{lemma}
\begin{lemma}
	
	$$\mu\qty(\qty(\min\left\{f,k \right\}) \cdot  \mathds{1}_{\frac{1}{k}\leq f}) \to \mu(f)$$
	\begin{proof}
		Given $\phi \in S^+$, $\phi \leq f$, for $k$ large enough, $\phi \leq \qty(\min\left\{f,k \right\}) \cdot  \mathds{1}_{\frac{1}{k}\leq f}$.  Since $\phi = \sum_{l=1}^m a_l \mathds{1}_{A_l} $ $\phi \leq f\cdot  \mathds{1}_{\frac{1}{k}\leq f}$ and for $k$ large enough $\phi \leq \min\left\{f,k \right\}$. Thus 
		$$\phi \leq \qty(\min\left\{f,k \right\}) \cdot  \mathds{1}_{\frac{1}{k}\leq f}$$
		and
		$$\mu_0(\phi) \leq \mu\qty(\qty(\min\left\{f,k \right\}) \cdot  \mathds{1}_{\frac{1}{k}\leq f})$$
		Taking the limit
		$$\mu_0(\phi) \leq \lim_{k\to \infty} \mu\qty(\qty(\min\left\{f,k \right\}) \cdot  \mathds{1}_{\frac{1}{k}\leq f})$$
		By taking supremum over $\phi$
		$$\mu(f) \leq \lim_{k\to \infty} \mu\qty(\qty(\min\left\{f,k \right\}) \cdot  \mathds{1}_{\frac{1}{k}\leq f})$$
		Other direction is trivial and thus
		$$\mu\qty(\qty(\min\left\{f,k \right\}) \cdot  \mathds{1}_{\frac{1}{k}\leq f}) \to \mu(f)$$
	\end{proof}
\end{lemma}
\begin{theorem}[Monotone convergence theorem] \label{mct}
	Let $0<f_n$ and $f_n\uparrow f$, then $\mu(f_n) \uparrow \mu(f)$
	
	\begin{proof}
		From lemma we can assume $f$ is bonded and 
		$$\exists \epsilon \quad \left\{ f>0\right\}=\left\{ f>\epsilon\right\}$$
		
		If $\mu(f>\epsilon) = \infty$, then $\mu(f) = \infty$. Also
		$$\left\{ f_n > \frac{\epsilon}{2} \right\} \uparrow \left\{ f \geq \frac{\epsilon}{2} \right\} \Rightarrow \mu\qty(f_n > \frac{\epsilon}{2}) \to \mu\qty(f\geq)\frac{\epsilon}{2})$$
		Thus $\mu(f_n>\epsilon) \to \infty$
		
		If $\mu(f>\epsilon) < \infty$, given $\delta>0$, let
		$$C_n = \left\{ \abs{f-f_n} > \delta, f>\epsilon \right\}$$
		Then $C_n \downarrow \emptyset$, thus $\forall \delta>0$ $\mu(C_n) \to 0$.
		
		Given $S \ni \phi \leq f$, $$\phi = \phi \mathds{1}_{f>\epsilon} = (\phi-\delta) \mathds{1}_{f>\epsilon} + \delta \mathds{1}_{f>\epsilon}$$
		Let $\phi_n = (\phi-\delta) \mathds{1}_{f>\epsilon}\mathds{1}_{\abs{f-f_n}<\delta}$. Obviously $\phi_n\leq f_n$.
		
		We claim
		$$\exists C>0 \quad \abs{\mu_0(\phi_n) - \mu_0(\phi)} \leq C\cdot \qty(\delta + \mu(C_n))$$
		since
		$$\mu_0(\phi_n) = \mu_0(\phi) - \delta\mu\qty(f>\epsilon, \abs{f-f_n}>\delta) - \delta \mu(f>\epsilon)$$
		$$\abs{\mu_0(\phi_n) - \mu_0(\phi)} \leq \delta \mu(f>\epsilon) + M\mu(C_n)$$
		for $M\geq f$.
		
		Since $\delta$ is arbitrary, $\lim_{n\to \infty} C\cdot \qty(\delta + \mu(C_n)) = 0$, thus
		$$\mu_0(\phi) \leq \lim_{n\to \infty} \mu_0(f_n) $$
		
		Optimizing over $\phi$ we get
		$$\mu(f) \leq \lim_{n\to \infty} \mu(f_n)$$
	\end{proof}
\begin{coll}
	$f,g\in \mathcal{P}$ and $a\geq 0$ then
	$$\mu(af+g) = a\mu(f)+\mu(g)$$
	\begin{proof}
		Taking staircase functions $\alpha^{(r)}_f$ and $\alpha^{(r)}_g$. Then $a\alpha^{(r)}_f+ \alpha^{(r)}_g \uparrow af+g$ and
		$$\mu\qty(a\alpha^{(r)}_f+ \alpha^{(r)}_g) = a\mu\qty(\alpha^{(r)}_f) + \mu\qty(\alpha^{(r)}_g)$$
		By \ref{mct}
		$$\lim_{r\to \infty} \mu\qty(a\alpha^{(r)}_f+ \alpha^{(r)}_g) = \lim_{r\to \infty}  a\mu\qty(\alpha^{(r)}_f) + \mu\qty(\alpha^{(r)}_g)$$
		$$\mu(af+g) = a\mu(f)+\mu(g)$$
	\end{proof}
\end{coll}
\begin{coll}
$$\mu\qty(\liminf f_n) \leq \liminf \mu(f_n)$$
\begin{proof}
	$$\liminf f_n = \sup\limits_k \qty[\underbrace{\inf\limits_{n\geq k} f_n}_{g_k}] $$
	$$g_k \uparrow \liminf f_n$$
	From \ref{mct}
	$$\mu(\liminf f_n) = \lim_{k} \mu(g_k) \leq \liminf_k \mu(f_k)$$
\end{proof}
\end{coll}
\end{theorem}